@prefix : <http://www.w3.org/2002/07/owl#> .
@prefix owl: <http://www.w3.org/2002/07/owl#> .
@prefix pmo: <https://juandql.github.io/ontologies/parking-multicoding/> .
@prefix rdf: <http://www.w3.org/1999/02/22-rdf-syntax-ns#> .
@prefix xml: <http://www.w3.org/XML/1998/namespace> .
@prefix xsd: <http://www.w3.org/2001/XMLSchema#> .
@prefix rdfs: <http://www.w3.org/2000/01/rdf-schema#> .
@base <http://whttps://juandql.github.io/ontologies/parking-multicoding#> .

<https://juandql.github.io/ontologies/parking-multicoding> rdf:type owl:Ontology ;
                                                            <http://purl.org/dc/elements/1.1/description> """An ontology about street parking spots in Berlin, describing their properties and attributes, with focus on the multicoding (re-purposing) of those spots. Based on the three datasets from the Berlin Open Data initiative:

(1) Street Parking Spots inside Berlin's S-Bahn-Ring (see https://gdi.berlin.de/geonetwork/srv/ger/catalog.search#/metadata/3c507d6f-77d6-48bd-aa9b-0d6b3ed1d894)
(2) Road Sections - Traffic Components of the regional reference system (RBS) (see https://gdi.berlin.de/geonetwork/srv/ger/catalog.search#/metadata/6bdd6d60-9e41-4fd1-afef-c872b6679643)
(3) Traffic Speed Limits (see https://gdi.berlin.de/geonetwork/srv/ger/catalog.search#/metadata/609fb162-892d-301c-9aa6-331dd44f5a7a)"""@en ,
                                                                                                          "Creative Commons Attribution 3.0 (CC BY 3.0)" ,
                                                                                                          "Juan de Queiroz Leles" ;
                                                            <http://purl.org/dc/elements/1.1/title> "parking multicoding ontology"@en ;
                                                            <http://purl.org/dc/terms/provenance> """v1.0: first ontology for parking multicoding

v2.0: Removing the class 'Street' and replacing it with an object property 'withinStreet'. Change of domain from properties 'hasSpeedLimit' and 'hasStreetID' to the class 'StreetParkingSpotGroup\". Addition of new property 'hasRestrictedDays' and 'withinDistrict'""" ;
                                                            rdfs:label "parking multicoding"@en ;
                                                            owl:versionInfo "2.0" .

#################################################################
#    Annotation properties
#################################################################

###  http://purl.org/dc/elements/1.1/description
<http://purl.org/dc/elements/1.1/description> rdf:type owl:AnnotationProperty .


###  http://purl.org/dc/elements/1.1/title
<http://purl.org/dc/elements/1.1/title> rdf:type owl:AnnotationProperty .


###  http://purl.org/dc/terms/contributor
<http://purl.org/dc/terms/contributor> rdf:type owl:AnnotationProperty .


###  http://purl.org/dc/terms/license
<http://purl.org/dc/terms/license> rdf:type owl:AnnotationProperty .


###  http://purl.org/dc/terms/provenance
<http://purl.org/dc/terms/provenance> rdf:type owl:AnnotationProperty .


#################################################################
#    Object Properties
#################################################################

###  https://juandql.github.io/ontologies/parking-multicoding/allowsFunction
pmo:allowsFunction rdf:type owl:ObjectProperty ;
                   rdfs:domain pmo:ParkingCategory ;
                   rdfs:range pmo:ParkingSpotFunction ;
                   rdfs:comment "Object property describing the possible functions of the parking categories."@en ;
                   rdfs:label "allows function"@en .


###  https://juandql.github.io/ontologies/parking-multicoding/hasCategory
pmo:hasCategory rdf:type owl:ObjectProperty ;
                rdfs:domain pmo:StreetParkingSpotGroup ;
                rdfs:range pmo:ParkingCategory ;
                rdfs:comment "Object property associating the different categories that a street parking spot group can assume."@en ;
                rdfs:label "has category"@en .


###  https://juandql.github.io/ontologies/parking-multicoding/hasParkingOrientation
pmo:hasParkingOrientation rdf:type owl:ObjectProperty ;
                          rdfs:domain pmo:StreetParkingSpotGroup ;
                          rdfs:range pmo:ParkingOrientation ;
                          rdfs:comment "Object property associating the individuals of street parking spot group with their equivalent parking orientation (angled, parallel, perpendicular)."@en ;
                          rdfs:label "has parking orientation"@en .


###  https://juandql.github.io/ontologies/parking-multicoding/hasRestrictionReason
pmo:hasRestrictionReason rdf:type owl:ObjectProperty ;
                         rdfs:domain pmo:ParkingCategory ;
                         rdfs:range pmo:RestrictionReason ;
                         rdfs:comment "Object property associating the possible restriction reason of a given parking category."@en ;
                         rdfs:label "has restriction reason"@en .


###  https://juandql.github.io/ontologies/parking-multicoding/withinParkingSite
pmo:withinParkingSite rdf:type owl:ObjectProperty ;
                      rdfs:domain pmo:StreetParkingSpotGroup ;
                      rdfs:range pmo:ParkingSite ;
                      rdfs:comment "Object property associating a street parking spot group with its physical location within a public street (parking by, full or half over a sidewalk, over lane)."@en ;
                      rdfs:label "within parking site"@en .


#################################################################
#    Data properties
#################################################################

###  https://juandql.github.io/ontologies/parking-multicoding/hasChargingStation
pmo:hasChargingStation rdf:type owl:DatatypeProperty ;
                       rdfs:domain pmo:ParkingCategory ;
                       rdfs:range xsd:boolean ;
                       rdfs:comment "Data property associating a boolean value to the individuals of the class ParkingCategory. An individual with value 'true' is adapted for electrical vehicle parking. This property is built to follow the structure of the dataset of street parking spots from Berlin."@en ;
                       rdfs:label "has charging station"@en .


###  https://juandql.github.io/ontologies/parking-multicoding/hasNumberOfSpots
pmo:hasNumberOfSpots rdf:type owl:DatatypeProperty ;
                     rdfs:domain pmo:StreetParkingSpotGroup ;
                     rdfs:range xsd:integer ;
                     rdfs:comment "Data property associating a number (integer) to the individuals of the class StreetParkingSpotGroup. This number represents how many spots are in a given parking spot group. This property is built to follow the structure of the dataset of street parking spots from Berlin."@en ;
                     rdfs:label "has number of spots"@en .


###  https://juandql.github.io/ontologies/parking-multicoding/hasParkingGroupID
pmo:hasParkingGroupID rdf:type owl:DatatypeProperty ;
                      rdfs:domain pmo:StreetParkingSpotGroup ;
                      rdfs:range xsd:integer ;
                      rdfs:comment "Data property associating a number (integer) to the individuals of the class StreetParkingSpotGroup, as a unique individual identifier. This property is built to follow the structure of the dataset of street parking spots from Berlin Open Data."@en ;
                      rdfs:label "has parking group id"@en .


###  https://juandql.github.io/ontologies/parking-multicoding/hasRestrictedDays
pmo:hasRestrictedDays rdf:type owl:DatatypeProperty ;
                      rdfs:domain pmo:StreetParkingSpotGroup ;
                      rdfs:range xsd:string ;
                      rdfs:comment "Data property associating a string value (list of days of the week) to the individuals of the class StreetParkingSpotGroup. This property is built to follow the structure of the dataset of street parking spots from Berlin, where some parking spots have a restriction reason with a time validity."@en ;
                      rdfs:label "has restricted days"@en .


###  https://juandql.github.io/ontologies/parking-multicoding/hasSpeedLimit
pmo:hasSpeedLimit rdf:type owl:DatatypeProperty ;
                  rdfs:domain pmo:StreetParkingSpotGroup ;
                  rdfs:range xsd:integer ;
                  rdfs:comment "Data property associating a number (integer) to the individuals of the class StreetParkingSpotGroup. This number represents the traffic speed limit of the street where the parking spot group is located. This property is built based on the data retrieved in the dataset  called Tempolimit from Berlin Open Data."@en ;
                  rdfs:label "has speed limit"@en .


###  https://juandql.github.io/ontologies/parking-multicoding/hasStreetID
pmo:hasStreetID rdf:type owl:DatatypeProperty ;
                rdfs:domain pmo:StreetParkingSpotGroup ;
                rdfs:range xsd:string ;
                rdfs:comment "Data property associating a number (integer) to the individuals of the class StreetParkingSpotGroup. This number represents the unique identifier of streets, where the parking spot group is located. This property is built based on the data retrieved in  the dataset Stra√üenabschnitte (RBS) from Berlin Open Data."@en ;
                rdfs:label "has street id"@en .


###  https://juandql.github.io/ontologies/parking-multicoding/isUniversallyAccessible
pmo:isUniversallyAccessible rdf:type owl:DatatypeProperty ;
                            rdfs:domain pmo:ParkingCategory ;
                            rdfs:range xsd:boolean ;
                            rdfs:comment "Data property associating a boolean value to the individuals of the class ParkingCategory. An individual with value 'true' is universally accessible. This property is built to follow the structure of the dataset of street parking spots from Berlin."@en ;
                            rdfs:label "is universally accessible"@en .


###  https://juandql.github.io/ontologies/parking-multicoding/withinDistrict
pmo:withinDistrict rdf:type owl:DatatypeProperty ;
                   rdfs:domain pmo:StreetParkingSpotGroup ;
                   rdfs:range xsd:string ;
                   rdfs:comment "Data property associating a string to the individuals of the class StreetParkingSpotGroup. This string represents the name of the district where the parking spot group is located. This property is built based on the data retrieved in  the dataset Stra√üenabschnitte (RBS) from Berlin Open Data."@en ;
                   rdfs:label "within district"@en .


###  https://juandql.github.io/ontologies/parking-multicoding/withinParkingZone
pmo:withinParkingZone rdf:type owl:DatatypeProperty ;
                      rdfs:domain pmo:StreetParkingSpotGroup ;
                      rdfs:range xsd:string ;
                      rdfs:comment "Data property associating a string to the individuals of the class StreetParkingSpotGroup, representing the name/number of the given parking zone where the parking spot group is located. This property is built to follow the structure of the dataset of street parking spots from Berlin Open Data."@en ;
                      rdfs:label "wihitn parking zone"@en .


###  https://juandql.github.io/ontologies/parking-multicoding/withinStreet
pmo:withinStreet rdf:type owl:DatatypeProperty ;
                 rdfs:domain pmo:StreetParkingSpotGroup ;
                 rdfs:range xsd:string ;
                 rdfs:comment "Data property associating a string to the individuals of the class StreetParkingSpotGroup, representing the name of the street where the parking spot group is located. This property is built to follow the structure of the dataset of street parking spots from Berlin Open Data.e"@en ;
                 rdfs:label "within street"@en .


#################################################################
#    Classes
#################################################################

###  https://juandql.github.io/ontologies/parking-multicoding/AlternativeFunction
pmo:AlternativeFunction rdf:type owl:Class ;
                        rdfs:subClassOf pmo:ParkingSpotFunction ;
                        owl:disjointWith pmo:VehicleParkingFunction ;
                        rdfs:comment "A class representing the individuals that allows other functions to the street parking spots than traditional vehicle parking. Those individuals are range for the object property 'allowsFunction'. Here alternative function is described in singular, but shall represent all the possible alternative functions that one could plan as a temporary use of a street parking spot (e.g. urban garden, terrace, street furniture, playground, etc.). This class was create to make explicit the disjonction with the class 'VehicleParkingFunction'." ;
                        rdfs:label "Alternative Function" .


###  https://juandql.github.io/ontologies/parking-multicoding/BusStopCategory
pmo:BusStopCategory rdf:type owl:Class ;
                    owl:equivalentClass [ rdf:type owl:Restriction ;
                                          owl:onProperty pmo:hasRestrictionReason ;
                                          owl:hasValue pmo:Bus-only_Lane
                                        ] ;
                    rdfs:subClassOf pmo:ParkingCategory ,
                                    [ rdf:type owl:Restriction ;
                                      owl:onProperty pmo:allowsFunction ;
                                      owl:hasValue pmo:Vehicle_Parking
                                    ] ;
                    rdfs:comment "A class that is equivalent to the set of individuals that has the value 'Bus-only lane' (de: Bussonderfahrstreifen) for the property 'hasRestrictionReason'. For the inidividuals of this class no alternative function is allowed, only for vehicle parking (in this case bus stop)." ;
                    rdfs:label "Bus Stop Category" .


###  https://juandql.github.io/ontologies/parking-multicoding/ElectricalVehicleCategory
pmo:ElectricalVehicleCategory rdf:type owl:Class ;
                              owl:equivalentClass [ rdf:type owl:Restriction ;
                                                    owl:onProperty pmo:hasChargingStation ;
                                                    owl:hasValue "true"^^xsd:boolean
                                                  ] ;
                              rdfs:subClassOf pmo:ParkingCategory ,
                                              [ rdf:type owl:Restriction ;
                                                owl:onProperty pmo:allowsFunction ;
                                                owl:hasValue pmo:Vehicle_Parking
                                              ] ;
                              owl:disjointWith pmo:GeneralCategory ,
                                               pmo:LoadZoneCategory ,
                                               pmo:UniversallyAccessibleCategory ;
                              rdfs:comment "A class that is equivalent to the set of individuals that has the value 'true'  for the property 'hasChargingStation', describing the set of parking spots for eletrical vehicles. For the inidividuals of this class no alternative function is allowed, only for vehicle parking." ;
                              rdfs:label "Eletrical Vehicles Category" .


###  https://juandql.github.io/ontologies/parking-multicoding/GeneralCategory
pmo:GeneralCategory rdf:type owl:Class ;
                    owl:equivalentClass [ owl:intersectionOf ( [ rdf:type owl:Restriction ;
                                                                 owl:onProperty pmo:hasRestrictionReason ;
                                                                 owl:hasValue pmo:No_Restriction_Reason
                                                               ]
                                                               [ rdf:type owl:Restriction ;
                                                                 owl:onProperty pmo:hasChargingStation ;
                                                                 owl:hasValue "false"^^xsd:boolean
                                                               ]
                                                               [ rdf:type owl:Restriction ;
                                                                 owl:onProperty pmo:isUniversallyAccessible ;
                                                                 owl:hasValue "false"^^xsd:boolean
                                                               ]
                                                             ) ;
                                          rdf:type owl:Class
                                        ] ;
                    rdfs:subClassOf pmo:ParkingCategory ,
                                    [ rdf:type owl:Restriction ;
                                      owl:onProperty pmo:allowsFunction ;
                                      owl:hasValue pmo:Alternative_Function
                                    ] ,
                                    [ rdf:type owl:Restriction ;
                                      owl:onProperty pmo:allowsFunction ;
                                      owl:hasValue pmo:Vehicle_Parking
                                    ] ;
                    owl:disjointWith pmo:LoadZoneCategory ,
                                     pmo:TaxiCategory ,
                                     pmo:UniversallyAccessibleCategory ;
                    rdfs:comment "A class that is equivalent to the set of individuals that has the value 'NoRestrictionReason' for the property 'hasRestrictionReason', AND that has the value 'false' similtaneously for the properties 'IsUniversallyAccessible' and 'hasChargingStation'. Meaning: the individuals of this class has no parking restriction, are neither adequate for electrical vehicles nor suitable for accessible parking. For the inidividuals of this class an alternative function is allowed, other then the original vehicle parking function." ;
                    rdfs:label "General Category" .


###  https://juandql.github.io/ontologies/parking-multicoding/LoadZoneCategory
pmo:LoadZoneCategory rdf:type owl:Class ;
                     owl:equivalentClass [ rdf:type owl:Restriction ;
                                           owl:onProperty pmo:hasRestrictionReason ;
                                           owl:hasValue pmo:Loading_Zone
                                         ] ;
                     rdfs:subClassOf pmo:ParkingCategory ,
                                     [ rdf:type owl:Restriction ;
                                       owl:onProperty pmo:allowsFunction ;
                                       owl:hasValue pmo:Vehicle_Parking
                                     ] ;
                     owl:disjointWith pmo:TaxiCategory ,
                                      pmo:UniversallyAccessibleCategory ;
                     rdfs:comment "A class that is equivalent to the set of individuals that has the value 'LoadingZone' (de: Ladezone) for the property 'hasRestrictionReason'. For the inidividuals of this class no alternative function is allowed, only for vehicle parking for loading and deloading goods." ;
                     rdfs:label "Load Zone Category" .


###  https://juandql.github.io/ontologies/parking-multicoding/OfficialVehicleCategory
pmo:OfficialVehicleCategory rdf:type owl:Class ;
                            owl:equivalentClass [ rdf:type owl:Restriction ;
                                                  owl:onProperty pmo:hasRestrictionReason ;
                                                  owl:hasValue pmo:Police_Vehicle-only
                                                ] ;
                            rdfs:subClassOf pmo:ParkingCategory ,
                                            [ rdf:type owl:Restriction ;
                                              owl:onProperty pmo:allowsFunction ;
                                              owl:hasValue pmo:Vehicle_Parking
                                            ] ;
                            rdfs:comment "A class that is equivalent to the set of individuals that has the value 'PoliceVehicleOnly' (de: Polizeifahrzeuge) for the property 'hasRestrictionReason'. For the inidividuals of this class no alternative function is allowed, only for police's vehicles parking." ;
                            rdfs:label "Official Vehicles Category" .


###  https://juandql.github.io/ontologies/parking-multicoding/ParkingCategory
pmo:ParkingCategory rdf:type owl:Class ;
                    rdfs:subClassOf [ rdf:type owl:Restriction ;
                                      owl:onProperty pmo:hasChargingStation ;
                                      owl:someValuesFrom xsd:boolean
                                    ] ,
                                    [ rdf:type owl:Restriction ;
                                      owl:onProperty pmo:isUniversallyAccessible ;
                                      owl:someValuesFrom xsd:boolean
                                    ] ;
                    rdfs:comment "A class that describes the street parking spots in 8 categories, based in the information provided by the dataset for street parking spots in Berlin. The categories are mainly related to the information provided by the fields 'restriction reason' (de: grund_fuer_beschraenkung), 'charging station' (de: ladesaeule) and 'universally accessible' (de: nur_schwerbehindert)." ;
                    rdfs:label "Parking Category"@en .


###  https://juandql.github.io/ontologies/parking-multicoding/ParkingOrientation
pmo:ParkingOrientation rdf:type owl:Class ;
                       rdfs:comment "" ,
                                    "A class for the inviduals describing the three possible street parking spot orientation (de: ausrichtung): angled parking, parallel parking and perpendicular parking." ;
                       rdfs:label "Parking Orientation" .


###  https://juandql.github.io/ontologies/parking-multicoding/ParkingSite
pmo:ParkingSite rdf:type owl:Class ;
                rdfs:comment "A class for the inviduals describing the four possible sites or locations within the public space in Berlin (de: parkort) of a given street parking spot : over a parking bay, full sidewalk, half sidewalk or over lane." ;
                rdfs:label "Parking Site" .


###  https://juandql.github.io/ontologies/parking-multicoding/ParkingSpotFunction
pmo:ParkingSpotFunction rdf:type owl:Class ;
                        rdfs:comment "A class containing two subclasses: AlternativeFunction and VehicleParkingFunction. This class describes the two possible functions of a street parking spot (vehicle parking and alternative function) and allows the attribution of those functions in relation to the class 'ParkingCategory' and its axioms." ;
                        rdfs:label "Parking Spot Function" .


###  https://juandql.github.io/ontologies/parking-multicoding/RestrictionReason
pmo:RestrictionReason rdf:type owl:Class ;
                      rdfs:comment "A class with all the individuals representing the different restriction reasons (de: grund fuer beschraenkung) of a given street parking spot, according to Berlin's dataset for parking spots. This class is range for the property 'hasRestrictionReason'." ;
                      rdfs:label "Restriction Reason" .


###  https://juandql.github.io/ontologies/parking-multicoding/StreetParkingSpotGroup
pmo:StreetParkingSpotGroup rdf:type owl:Class ;
                           rdfs:subClassOf [ rdf:type owl:Restriction ;
                                             owl:onProperty pmo:hasCategory ;
                                             owl:someValuesFrom pmo:ParkingCategory
                                           ] ,
                                           [ rdf:type owl:Restriction ;
                                             owl:onProperty pmo:hasParkingOrientation ;
                                             owl:someValuesFrom pmo:ParkingOrientation
                                           ] ,
                                           [ rdf:type owl:Restriction ;
                                             owl:onProperty pmo:hasRestrictionReason ;
                                             owl:someValuesFrom pmo:RestrictionReason
                                           ] ,
                                           [ rdf:type owl:Restriction ;
                                             owl:onProperty pmo:withinParkingSite ;
                                             owl:someValuesFrom pmo:ParkingSite
                                           ] ,
                                           [ rdf:type owl:Restriction ;
                                             owl:onProperty pmo:hasNumberOfSpots ;
                                             owl:someValuesFrom xsd:integer
                                           ] ,
                                           [ rdf:type owl:Restriction ;
                                             owl:onProperty pmo:hasParkingGroupID ;
                                             owl:someValuesFrom xsd:integer
                                           ] ,
                                           [ rdf:type owl:Restriction ;
                                             owl:onProperty pmo:hasRestrictedDays ;
                                             owl:someValuesFrom xsd:string
                                           ] ,
                                           [ rdf:type owl:Restriction ;
                                             owl:onProperty pmo:hasSpeedLimit ;
                                             owl:someValuesFrom xsd:integer
                                           ] ,
                                           [ rdf:type owl:Restriction ;
                                             owl:onProperty pmo:hasStreetID ;
                                             owl:someValuesFrom xsd:string
                                           ] ,
                                           [ rdf:type owl:Restriction ;
                                             owl:onProperty pmo:withinDistrict ;
                                             owl:someValuesFrom xsd:string
                                           ] ,
                                           [ rdf:type owl:Restriction ;
                                             owl:onProperty pmo:withinParkingZone ;
                                             owl:someValuesFrom xsd:string
                                           ] ,
                                           [ rdf:type owl:Restriction ;
                                             owl:onProperty pmo:withinStreet ;
                                             owl:someValuesFrom xsd:string
                                           ] ;
                           rdfs:comment "A class for describing all the individuals that can be found in the Berlin Dataset for street parking spots. Following the structure of the dataset, individuals of this class can represent parking spots with a single spot, as well of parking spots with multiple spots, therefore the name parking spots 'group'." ;
                           rdfs:label "Street Parking Spot Group" .


###  https://juandql.github.io/ontologies/parking-multicoding/TaxiCategory
pmo:TaxiCategory rdf:type owl:Class ;
                 owl:equivalentClass [ rdf:type owl:Restriction ;
                                       owl:onProperty pmo:hasRestrictionReason ;
                                       owl:hasValue pmo:Taxi-only
                                     ] ;
                 rdfs:subClassOf pmo:ParkingCategory ,
                                 [ rdf:type owl:Restriction ;
                                   owl:onProperty pmo:allowsFunction ;
                                   owl:hasValue pmo:Vehicle_Parking
                                 ] ;
                 owl:disjointWith pmo:UniversallyAccessibleCategory ;
                 rdfs:comment "A class that is equivalent to the set of individuals that has the value 'TaxiOnly' (de: Taxi) for the property 'hasRestrictionReason'. For the inidividuals of this class no alternative function is allowed, only for the parking of taxis-." ;
                 rdfs:label "Taxi Category" .


###  https://juandql.github.io/ontologies/parking-multicoding/UniversallyAccessibleCategory
pmo:UniversallyAccessibleCategory rdf:type owl:Class ;
                                  owl:equivalentClass [ rdf:type owl:Restriction ;
                                                        owl:onProperty pmo:isUniversallyAccessible ;
                                                        owl:hasValue "true"^^xsd:boolean
                                                      ] ;
                                  rdfs:subClassOf pmo:ParkingCategory ,
                                                  [ rdf:type owl:Restriction ;
                                                    owl:onProperty pmo:allowsFunction ;
                                                    owl:hasValue pmo:Vehicle_Parking
                                                  ] ;
                                  rdfs:comment "A class that is equivalent to the set of individuals that has the value 'true' for the property 'isUniversallyAccessible'. For the inidividuals of this class no alternative function is allowed, only for vehicle parking in spots adapted for universal accessibility." ;
                                  rdfs:label "Universally Acessible Category" .


###  https://juandql.github.io/ontologies/parking-multicoding/UnkownCategory
pmo:UnkownCategory rdf:type owl:Class ;
                   owl:equivalentClass [ rdf:type owl:Restriction ;
                                         owl:onProperty pmo:hasRestrictionReason ;
                                         owl:hasValue pmo:Other_Restriction
                                       ] ;
                   rdfs:subClassOf pmo:ParkingCategory ,
                                   [ rdf:type owl:Restriction ;
                                     owl:onProperty pmo:allowsFunction ;
                                     owl:hasValue pmo:Vehicle_Parking
                                   ] ;
                   rdfs:comment "A class that is equivalent to the set of individuals that has the value 'OtherRestriction' (de: Andere Beschraenkungen) for the property 'hasRestrictionReason'. Since no information is provided in the dataset for street parking spots from Berlin, it is assumed that for the inidividuals of this class no alternative function is allowed, only for vehicle parking." ;
                   rdfs:label "Unknow Category" .


###  https://juandql.github.io/ontologies/parking-multicoding/VehicleParkingFunction
pmo:VehicleParkingFunction rdf:type owl:Class ;
                           rdfs:subClassOf pmo:ParkingSpotFunction ;
                           rdfs:comment "A class representing the individuals that allows only the original function of a street parking spots:  vehicle parking. Those individuals are range for the object property 'allowsFunction'. This class was create to make explicit the disjonction with the class 'AlternativeFunction'." ;
                           rdfs:label "Vehicle Parking Function" .


#################################################################
#    Individuals
#################################################################

###  https://juandql.github.io/ontologies/parking-multicoding/Alternative_Function
pmo:Alternative_Function rdf:type owl:NamedIndividual ,
                                  pmo:AlternativeFunction .


###  https://juandql.github.io/ontologies/parking-multicoding/Angled_Parking
pmo:Angled_Parking rdf:type owl:NamedIndividual ,
                            pmo:ParkingOrientation .


###  https://juandql.github.io/ontologies/parking-multicoding/Bus-only_Lane
pmo:Bus-only_Lane rdf:type owl:NamedIndividual ,
                           pmo:RestrictionReason .


###  https://juandql.github.io/ontologies/parking-multicoding/Full_Sidewalk_Parking
pmo:Full_Sidewalk_Parking rdf:type owl:NamedIndividual ,
                                   pmo:ParkingSite .


###  https://juandql.github.io/ontologies/parking-multicoding/Half_Sidewalk_Parking
pmo:Half_Sidewalk_Parking rdf:type owl:NamedIndividual ,
                                   pmo:ParkingSite .


###  https://juandql.github.io/ontologies/parking-multicoding/Lane_Parking
pmo:Lane_Parking rdf:type owl:NamedIndividual ,
                          pmo:ParkingSite .


###  https://juandql.github.io/ontologies/parking-multicoding/Loading_Zone
pmo:Loading_Zone rdf:type owl:NamedIndividual ,
                          pmo:RestrictionReason .


###  https://juandql.github.io/ontologies/parking-multicoding/No_Restriction_Reason
pmo:No_Restriction_Reason rdf:type owl:NamedIndividual ,
                                   pmo:RestrictionReason .


###  https://juandql.github.io/ontologies/parking-multicoding/Other_Restriction
pmo:Other_Restriction rdf:type owl:NamedIndividual ,
                               pmo:RestrictionReason .


###  https://juandql.github.io/ontologies/parking-multicoding/Parallel_Parking
pmo:Parallel_Parking rdf:type owl:NamedIndividual ,
                              pmo:ParkingOrientation .


###  https://juandql.github.io/ontologies/parking-multicoding/Parking_Bay
pmo:Parking_Bay rdf:type owl:NamedIndividual ,
                         pmo:ParkingSite .


###  https://juandql.github.io/ontologies/parking-multicoding/Perpendicular_Parking
pmo:Perpendicular_Parking rdf:type owl:NamedIndividual ,
                                   pmo:ParkingOrientation .


###  https://juandql.github.io/ontologies/parking-multicoding/Police_Vehicle-only
pmo:Police_Vehicle-only rdf:type owl:NamedIndividual ,
                                 pmo:RestrictionReason .


###  https://juandql.github.io/ontologies/parking-multicoding/Taxi-only
pmo:Taxi-only rdf:type owl:NamedIndividual ,
                       pmo:RestrictionReason .


###  https://juandql.github.io/ontologies/parking-multicoding/Vehicle_Parking
pmo:Vehicle_Parking rdf:type owl:NamedIndividual ,
                             pmo:VehicleParkingFunction .


###  Generated by the OWL API (version 4.5.29.2024-05-13T12:11:03Z) https://github.com/owlcs/owlapi
